TheoremsAboutAlgorithms/Partitions/WithFinset/Split.lean
@@ -1,0 +1,566 @@
+import Mathlib.Data.SetLike.Basic
+import Mathlib.Data.Setoid.Partition
+import TheoremsAboutAlgorithms.Partitions.WithFinset.Defs
+import TheoremsAboutAlgorithms.Partitions.WithFinset.Cell
+
+namespace Split
+
+def cast {n m : ℕ} (h : n = m) (split : Split n) : Split m
+  := Finset.map (Cell.castEmbedding h) split
+
+theorem cast_empty_not_mem_iff {n m : ℕ} (h : n = m) (split : Split n)
+  : ∅ ∉ split.cast h ↔ ∅ ∉ split := by
+    constructor <;> intro _ _ <;> simp [cast, Cell.castEmbedding, Cell.cast] at * <;> contradiction
+
+-- TODO: Fix the proof
+theorem cast_mem_iff {n : ℕ} (split : Split n) (cell : Cell n)
+  : cell ∈ split.cast rfl ↔ cell ∈ split := by
+    sorry
+    -- constructor <;> intro <;> simp [cast, Cell.castEmbedding, Cell.cast, Fin.castEmbedding] at * <;> assumption
+
+theorem cast_nonempty_iff {n m : ℕ} (h : n = m) (split : Split n)
+  : (split.cast h).Nonempty ↔ split.Nonempty := by simp [cast]
+
+def castSucc {n : ℕ} (split : Split n) : Split (n + 1)
+  := Cell.castSucc '' split
+
+theorem castSucc_injective {n : ℕ} : Function.Injective (castSucc (n := n)) := by
+  intro x y h
+  simp [castSucc] at h
+  have Cell.castSucc_injective_on_split := Function.Injective.image_injective (Cell.castSucc_injective (n := n))
+  exact Cell.castSucc_injective_on_split h
+
+-- TODO: Fix naming elem -> mem
+theorem castSucc_empty_elem_iff {n : ℕ} (split : Split n)
+  : ∅ ∈ split.castSucc ↔ ∅ ∈ split := by simp [castSucc, Cell.castSucc]
+
+-- TODO: This is more general than last_not_mem_of_mem_removeCell_castSucc right? We don't need the other one
+-- TODO: Rename, the naming seems of no? Should be last_not_mem_of_mem_castSucc?
+theorem castSucc_last_not_mem_of_mem {n : ℕ} {split : Split n} {cell : Cell (n + 1)} (h : cell ∈ split.castSucc)
+  : Fin.last n ∉ cell := by
+    simp [castSucc, Cell.castSucc] at h
+    cases h with
+      | intro cell_pre h_cell_pre =>
+        rw [← h_cell_pre.right]
+        simp
+        intro x _
+        exact Fin.ne_of_lt (Fin.castSucc_lt_last x)
+
+def removeCell {n : ℕ} (split : Split n) (cell : Cell n) : Split n
+  := split \ singleton cell
+
+-- TODO: Maybe we can find a better name yet (it's alright, but not totally satisfactory).
+-- We don't require targetCell ∈ split, because we want to be able to have ∅ as a target cell as well.
+-- This is essentially split ↦ {targetCell.transform} ∪ (split \ {targetCell})
+def insertLastAt {n : ℕ} (split : Split n) (targetCell : Cell n) : Split (n + 1)
+  := insert (targetCell.insertLast) (split.removeCell targetCell).castSucc
+
+------------------------------------------------------------------------------------------------------------------------
+--                                          Injectivity of insertLastAt                                               --
+------------------------------------------------------------------------------------------------------------------------
+
+theorem insertLastAt_injOn_helper_generalized_subset_helper
+    {n : ℕ}
+    {cell otherCell : Cell n}
+    {split otherSplit : Split (n + 1)}
+    (split'_eq_otherSplit' : insert cell.insertLast split = insert otherCell.insertLast otherSplit)
+    (last_not_mem_of_mem_split : ∀ cell, cell ∈ split → Fin.last n ∉ cell)
+  : split ⊆ otherSplit := by
+    intro x x_mem_split
+    have x_mem_insert_insertLast_otherCell_otherSplit : x ∈ insert otherCell.insertLast otherSplit := by
+      rw [← split'_eq_otherSplit']; simp; right; exact x_mem_split
+    cases x_mem_insert_insertLast_otherCell_otherSplit with
+      | inl x_eq_insertLast_otherCell =>
+        have last_mem_x := Cell.last_mem_insertLast otherCell
+        rw [← x_eq_insertLast_otherCell] at last_mem_x
+        have last_not_mem_x := last_not_mem_of_mem_split x x_mem_split
+        contradiction
+      | inr x_mem_otherSplit => exact x_mem_otherSplit
+
+-- TODO: NAMING!
+theorem insertLastAt_injOn_helper_generalized
+    {n : ℕ}
+    {cell otherCell : Cell n}
+    {split otherSplit : Split (n + 1)}
+    (split'_eq_otherSplit' : insert cell.insertLast split = insert otherCell.insertLast otherSplit)
+    (last_not_mem_of_mem_split : ∀ cell, cell ∈ split → Fin.last n ∉ cell)
+    (last_not_mem_of_mem_otherSplit : ∀ cell, cell ∈ otherSplit → Fin.last n ∉ cell)
+  : split = otherSplit := by
+    -- TODO: We know that insertLast is injective, use it here!
+    -- TODO: Totally symmetric, can we wlog it?
+    apply Set.eq_of_subset_of_subset
+    · exact insertLastAt_injOn_helper_generalized_subset_helper split'_eq_otherSplit' last_not_mem_of_mem_split
+    · exact insertLastAt_injOn_helper_generalized_subset_helper
+        split'_eq_otherSplit'.symm last_not_mem_of_mem_otherSplit
+
+theorem insertLastAt_injOn_helper
+    {n : ℕ}
+    {cell otherCell : Cell n}
+    {split : Split n}
+    (h : insert cell.insertLast (split.removeCell cell).castSucc
+          = insert otherCell.insertLast (split.removeCell otherCell).castSucc)
+  : (split.removeCell cell).castSucc = (split.removeCell otherCell).castSucc := by
+    have last_not_mem_of_mem_split' : ∀ x, x ∈ (split.removeCell cell).castSucc → Fin.last n ∉ x
+      := by intro _ x_mem_split'; exact castSucc_last_not_mem_of_mem x_mem_split'
+    have last_not_mem_of_mem_otherSplit' : ∀ x, x ∈ (split.removeCell otherCell).castSucc → Fin.last n ∉ x
+      := by intro _ x_mem_split'; exact castSucc_last_not_mem_of_mem x_mem_split'
+    exact insertLastAt_injOn_helper_generalized h last_not_mem_of_mem_split' last_not_mem_of_mem_otherSplit'
+
+-- TODO: Proof it
+theorem insertLastAt_injOn_disjoint_helper
+    {n : ℕ}
+    (x y : Cell n)
+    (split : Split n)
+  : Disjoint {x.insertLast} (split.removeCell y).castSucc := by
+    simp
+    have last_mem_insertLast_x := Cell.last_mem_insertLast x
+    have last_not_mem_of_mem_split' : ∀ cell, cell ∈ (split.removeCell y).castSucc → (Fin.last _) ∉ cell
+      := by intro cell cell_mem_split'; exact castSucc_last_not_mem_of_mem cell_mem_split'
+    intro insertLast_x_mem_split'
+    have last_not_mem_insertLast_x := last_not_mem_of_mem_split' x.insertLast insertLast_x_mem_split'
+    contradiction
+
+theorem insertLastAt_injOn_symmetric_case_helper
+    {n : ℕ}
+    {split : Split n}
+    {x y : Cell n}
+    (insertLastAt_x_eq_insertLastAt_y : split.insertLastAt x = split.insertLastAt y)
+    (x_eq_empty : x = ∅)
+  : x = y := by
+    -- TODO: Do we need all these have's? We can probably get rid of some of them
+    have singleton_last_mem_split'_x : {Fin.last _} ∈ split.insertLastAt x := by
+      simp [x_eq_empty, insertLastAt, Set.insert, Cell.insertLast, Cell.castSucc]
+        at insertLastAt_x_eq_insertLastAt_y ⊢
+    have singleton_last_mem_split'_y : {Fin.last _} ∈ split.insertLastAt y := by
+      rw [← insertLastAt_x_eq_insertLastAt_y]
+      exact singleton_last_mem_split'_x
+    have singleton_last_eq_y_insertLast : {Fin.last _} = y.insertLast := by
+      simp [insertLastAt, Cell.insertLast] at singleton_last_mem_split'_y
+      cases singleton_last_mem_split'_y with
+        | inl singleton_last_mem_set_insert =>
+          simp [Cell.insertLast]
+          exact singleton_last_mem_set_insert
+        | inr singleton_last_mem_removeCell =>
+          have := castSucc_last_not_mem_of_mem singleton_last_mem_removeCell
+          contradiction
+    have y_eq_empty : y = ∅ := by
+      simp [Cell.insertLast] at singleton_last_eq_y_insertLast
+      -- For some reason simp times out if we use it there
+      rw [Set.insert_eq (Fin.last n) (Cell.castSucc y)] at singleton_last_eq_y_insertLast
+      have castSucc_y_subset_singleton_last : Cell.castSucc y ⊆ {Fin.last _} := by
+        rw [singleton_last_eq_y_insertLast]
+        exact Set.subset_union_right _ _
+      have castSucc_y_Subsingleton : Set.Subsingleton (Cell.castSucc y)
+        := Set.subsingleton_of_subset_singleton castSucc_y_subset_singleton_last
+      have := Set.Subsingleton.eq_empty_or_singleton castSucc_y_Subsingleton
+      cases this with
+        | inl y_eq_empty => exact (Cell.castSucc_empty_iff y).mp y_eq_empty
+        | inr y_eq_singleton =>
+          -- TODO: Naming
+          obtain ⟨y_mem, y_mem_def⟩ := y_eq_singleton
+          have y_mem_eq_last : y_mem = Fin.last _ := by
+            rw [y_mem_def] at castSucc_y_subset_singleton_last
+            simp at castSucc_y_subset_singleton_last
+            exact castSucc_y_subset_singleton_last
+          have y_mem_ne_last : y_mem ≠ Fin.last _ := by
+            have exists_castSucc_eq_y_mem : ∃ (y' : Fin n), y'.castSucc = y_mem := by
+              rw [y_mem_eq_last]
+              simp [Cell.castSucc, Set.image] at y_mem_def
+              have : ∃ a ∈ y, Fin.castSucc a = y_mem := by
+                have : y_mem ∈ {x | ∃ a ∈ y, Fin.castSucc a = x} := by
+                  have := Set.mem_singleton y_mem
+                  rw [← y_mem_def] at this
+                  exact this
+                exact Set.mem_setOf.mp this
+              rw [y_mem_eq_last] at this
+              obtain ⟨y', _, y'_eq_y_mem⟩ := this
+              exists y'
+            exact Fin.exists_castSucc_eq.mp exists_castSucc_eq_y_mem
+          contradiction
+    rw [x_eq_empty, y_eq_empty]
+
+theorem insertLastAt_injOn {n : ℕ} (split : Split n)
+  : Set.InjOn (split.insertLastAt) (split.insert ∅) := by
+    intros x x_mem_split' y y_mem_split' insertLastAt_x_eq_insertLastAt_y
+    cases x_mem_split' with
+      | inl x_eq_empty =>
+        cases y_mem_split' with
+          | inl y_eq_empty => rw [x_eq_empty, y_eq_empty]
+          | inr y_mem_split =>
+            exact insertLastAt_injOn_symmetric_case_helper insertLastAt_x_eq_insertLastAt_y x_eq_empty
+      | inr x_mem_split =>
+        cases y_mem_split' with
+          | inl y_eq_empty =>
+            exact (insertLastAt_injOn_symmetric_case_helper insertLastAt_x_eq_insertLastAt_y.symm y_eq_empty).symm
+          | inr y_mem_split =>
+            simp [insertLastAt] at insertLastAt_x_eq_insertLastAt_y
+            have castSucc_eq : (split.removeCell x).castSucc = (split.removeCell y).castSucc
+              := insertLastAt_injOn_helper insertLastAt_x_eq_insertLastAt_y
+            rw [castSucc_eq] at insertLastAt_x_eq_insertLastAt_y
+            repeat rw [Set.insert_eq] at insertLastAt_x_eq_insertLastAt_y
+            -- TODO: There's probably a more straightforward way to do this
+            have singleton_insertLast_x_subset_y_union : {Cell.insertLast x} ⊆ {Cell.insertLast y} ∪ castSucc (removeCell split y) := by
+              have := Set.subset_union_left {Cell.insertLast x} (castSucc (split.removeCell y))
+              rw [insertLastAt_x_eq_insertLastAt_y] at this
+              exact this
+            have singleton_insertLast_x_subsetsingleton_insertLast_y : {Cell.insertLast x} ⊆ ({Cell.insertLast y} : (Split (n + 1))) := by
+              have singleton_insertLast_x_disjoint_castSucc := insertLastAt_injOn_disjoint_helper x y split
+              exact Disjoint.subset_left_of_subset_union singleton_insertLast_x_subset_y_union singleton_insertLast_x_disjoint_castSucc
+            have : Cell.insertLast x = Cell.insertLast y := by
+              apply Set.singleton_subset_singleton.mp
+              exact singleton_insertLast_x_subsetsingleton_insertLast_y
+            exact Cell.insertLast_injective this
+
+------------------------------------------------------------------------------------------------------------------------
+--                          Bijections between split₀ and split.insertLastAt targetCell                               --
+------------------------------------------------------------------------------------------------------------------------
+
+-- WIP (I)
+
+-- TODO: Injectivity of split.insertLastAt (as proved above) is not what we actually need in
+--       `isPartition_of_mem_insertLast'_of_isPartition`. What we do need are functions f g such that
+--
+--          `f : split₀ → split.insertLastAt targetCell`
+--          `g : split.insertLastAt targetCell → split₀`
+--
+--       and `f ∘ g = id` and `g ∘ f = id`. We want to define them as follows:
+--
+--          `f := if cell = targetCell then cell.insertLast else cell.castSucc`
+--          `g := if cell = targetCell.insertLast then targetCell else cell.castPred`
+--
+--       To do that computably we need instances for `DecidableEq Cell`, which we will get by reimplementing `Cell` via
+--       `Finset`. To see that what we plan to use them for [WIP (II)] works, we do it non-computably for now.
+
+-- Alternative definitions 2
+
+-- WIP (I.III)
+--    * Here we move the restrictions on the source and target domain of f and g from the types into the propositions,
+--      because right now it's kind of hard to get the types right (and this is intended to be a mere POC anyway)
+--    * Otherwise, we do the same as in WIP (I.II)
+
+theorem exists_f' {n : ℕ} (split : Split n) (targetCell : Cell n)
+  : ∃ (f : Cell n → Cell (n + 1)),
+    ∀ (cell : Cell n), cell ∈ split.insert ∅ →
+      (cell = targetCell → f cell ∈ split.insertLastAt targetCell ∧ f cell = targetCell.insertLast)
+      ∧ (cell ≠ targetCell → f cell ∈ split.insertLastAt targetCell ∧ f cell = cell.castSucc) := by
+        sorry
+
+noncomputable def f' {n : ℕ} (split : Split n) (targetCell : Cell n) : Cell n → Cell (n + 1)
+  := (exists_f' split targetCell).choose
+
+theorem exists_g' {n : ℕ} (split : Split n) (targetCell : Cell n)
+  : ∃ (g : Cell (n + 1) → Cell n),
+    ∀ (cell : Cell (n + 1)), cell ∈ split.insertLastAt targetCell →
+      (cell = targetCell.insertLast → g cell ∈ split.insert ∅ ∧ g cell = targetCell)
+      ∧ (cell ≠ targetCell.insertLast → g cell ∈ split.insert ∅ ∧ g cell = cell.castPred sorry) := by
+        sorry
+
+noncomputable def g' {n : ℕ} (split : Split n) (targetCell : Cell n) : Cell (n + 1) → Cell n
+  := (exists_g' split targetCell).choose
+
+theorem leftInverse_f'_g' {n : ℕ} (split : Split n) (targetCell : Cell n)
+  : Function.LeftInverse (f' split targetCell) (g' split targetCell) := by
+    sorry
+
+theorem rightInverse_f'_g' {n : ℕ} (split : Split n) (targetCell : Cell n)
+  : Function.RightInverse (f' split targetCell) (g' split targetCell) := by
+    sorry
+
+-- TODO: Use Function.bijective_iff_has_inverse for these
+theorem bijective_f' {n : ℕ} (split : Split n) (targetCell : Cell n)
+  : Function.Bijective (f' split targetCell) := by
+    sorry
+
+theorem bijective_g' {n : ℕ} (split : Split n) (targetCell : Cell n)
+  : Function.Bijective (g' split targetCell) := by
+    sorry
+
+-- Alternative definitions
+
+-- WIP (I.II)
+--    * This should be the better approach, defining directly what f and g look like at the different value pattern.
+--    * We should then (non-constructively) be able to proof left- / right-inverse by using `eq_or_ne` and accessing the
+--      definition of the values of f and g at the different value patterns.
+--    * Can we use `CoeDep` [0] to show that `Cell.castSucc cell : ↑(split.insertLastAt targetCell)`?. The instance
+--      below looks like it should help but it doesn't. The problem probably is that we use it in a type and so we need
+--      `CoeSort`?
+--    * Maybe there's something wrong with our `CoeDep`, `test2` should work (we coerce a value right?), but it doesn't
+--
+--    [0] https://lean-lang.org/functional_programming_in_lean/type-classes/coercion.html#non-empty-lists-and-dependent-coercions
+
+def nonTarget {n : ℕ} (split : Split n) (targetCell : Cell n) : Split n
+  := removeCell (split.insert ∅) targetCell
+
+theorem coe_castSucc_cell
+    {n : ℕ}
+    (split : Split n)
+    (targetCell : Cell n)
+    (cell : ↑(split.nonTarget targetCell))
+  : Cell.castSucc cell ∈ split.insertLastAt targetCell := by
+    simp [insertLastAt, Set.insert, Cell.castSucc]
+    right
+    exists cell
+    sorry
+
+-- We would rather have `cell_ne_targetCell : ↑cell ≠ targetCell` here but we don't know how to make it so that the
+-- coercion can then be found below, so we directly put it into the cell's type.
+instance
+    {n : ℕ}
+    {split : Split n}
+    {targetCell : Cell n}
+    {cell : ↑(split.nonTarget targetCell)}
+  : CoeDep (Cell (n + 1)) (Cell.castSucc cell) ↑(split.insertLastAt targetCell) where
+    coe := by
+      use Cell.castSucc cell
+      exact coe_castSucc_cell split targetCell cell
+
+-- Here we state the definition of f via propostions, because for a direct definition we need decidable equality on
+-- Cell. We can then noncomputably choose a function that satisfies the propositions.
+-- theorem exists_f {n : ℕ} (split : Split n) (targetCell : Cell n)
+--   : ∃ (f : ↑(split.insert ∅) → ↑(split.insertLastAt targetCell)),
+--     ∀ (cell : ↑(split.insert ∅)), (cell = targetCell → f cell = targetCell.insertLast)
+--       -- We have to explicitly specify `Cell (n + 1)` here such that the dependent coercion specified above can be found
+--       ∧ (↑cell ∈ split.nonTarget targetCell → f cell = ↑(Cell.castSucc (↑cell : ↑(split.nonTarget targetCell)) : Cell (n + 1))) := by
+--       sorry
+
+theorem exists_f_g {n : ℕ} (split : Split n) (targetCell : Cell n)
+  : ∃ (f : ↑(split.insert ∅) → ↑(split.insertLastAt targetCell)),
+    ∃ (g : ↑(split.insertLastAt targetCell) → ↑(split.insert ∅)),
+    Function.LeftInverse f g ∧ Function.RightInverse f g := by
+      sorry
+
+noncomputable def f {n : ℕ} (split : Split n) (targetCell : Cell n)
+  : ↑(split.insert ∅) → ↑(split.insertLastAt targetCell) :=
+    (exists_f_g split targetCell).choose
+
+-- TODO: Fix, how do we get to choose on the second exists?
+noncomputable def g {n : ℕ} (split : Split n) (targetCell : Cell n)
+  : ↑(split.insertLastAt targetCell) → ↑(split.insert ∅) :=
+    (exists_f_g split targetCell).choose_spec.choose
+
+-- TODO: Show this (as an exercise)
+example {n : ℕ} (split : Split n) (targetCell : Cell n)
+  : Function.LeftInverse (f split targetCell) (g split targetCell)
+    := (exists_f_g split targetCell).choose_spec.choose_spec.left
+
+-- We don't need this. We can use it for `(tcast split ▸ targetCell)` if `targetCell : ↑(split.insert ∅)`, but we don't
+-- have to actually do this since there is `Set.instCoeSortSetType  {α : Type u} : CoeSort (Set α) (Type u)` which
+-- is the "Coercion from a set to the corresponding subtype." so we can just use `targetCell : split.insert ∅` in places
+-- where we `targetCell : Cell n` is expected.
+theorem tcast
+    {n : ℕ}
+    (split : Split n)
+  : ↑(Set.insert ∅ split) = Cell n := by
+    sorry
+
+-- This is just `Set.instCoSortSetType`, we don't need it.
+--instance {n : ℕ} {split : Split n} : CoeSort ↑(Set.insert ∅ split) (Cell n) where
+--  coe cell := cell
+
+-- TODO: Fix, this is wrong!
+theorem icast
+    {n : ℕ}
+    (split : Split n)
+    (targetCell : ↑(split.insert ∅))
+  : Cell (n + 1) = ↑(split.insertLastAt targetCell) := by
+  --: ↑(Cell.insertLast targetCell) = ↑(split.insertLastAt targetCell) := by
+    sorry
+
+--instance {n : ℕ} {split : Split n} {targetCell : ↑(split.insert ∅)} : CoeSort (Cell (n + 1)) ↑(split.insertLastAt targetCell) where
+--  coe cell := sorry
+
+-- WIP (I.I)
+--    * Can we get rid of icast? Do we need an instance for that?
+--      * What does this error mean if we uncomment the second instance:
+--        ```
+--        instance does not provide concrete values for (semi-)out-params
+--          CoeSort (Cell (n + 1)) ↑(insertLastAt ?split ↑?targetCell)
+--        ```
+--    * `icast` looks questionable, we cast a Cell to "the type of elements of a split", which we can't do in general,
+--      because the cell need not be in the split. We probably need something along those lines (or the reverse?):
+--      ```
+--      ↑(Cell.insertLast targetCell) = ↑(split.insertLastAt targetCell)
+--      ```
+
+theorem f_targetCell_eq_targetCell_insertLast_with_instances
+    {n : ℕ}
+    (split : Split n)
+    (targetCell : ↑(split.insert ∅))
+    : f split targetCell targetCell
+        = ((icast split targetCell ▸ Cell.insertLast targetCell)
+            : ↑(insertLastAt split targetCell))
+      := by sorry
+
+--theorem f_targetCell_eq_targetCell_insertLast
+--    {n : ℕ}
+--    (split : Split n)
+--    (targetCell : ↑(split.insert ∅))
+--    : f split (tcast split ▸ targetCell) targetCell
+--        = ((icast split targetCell ▸ Cell.insertLast (tcast split ▸ targetCell))
+--            : ↑(insertLastAt split (tcast split ▸ targetCell)))
+--      := by sorry
+
+------------------------------------------------------------------------------------------------------------------------
+--                                          insertLastAt, insertLast, ...                                             --
+------------------------------------------------------------------------------------------------------------------------
+
+theorem insertLastAt_nonempty {n : ℕ} (split : Split n) (targetCell : Cell n)
+  : (split.insertLastAt targetCell).Nonempty
+    := Set.insert_nonempty _ _
+
+-- TODO: Can we simplify this proof?
+theorem insertLastAt_empty_not_mem_of_empty_not_mem
+  {n : ℕ} (split : Split n) (targetCell : Cell n) (h : ∅ ∉ split) : ∅ ∉ split.insertLastAt targetCell := by
+    simp [insertLastAt]
+    intro h_empty_elem
+    cases h_empty_elem with
+      | inl h_elem_insertLast =>
+        have := Cell.insertLast_nonempty targetCell
+        -- TODO: There has to be an easier way to show Set.Nonempty x → ∅ = x → False
+        rw [← h_elem_insertLast] at this
+        cases this with
+          | intro x h_x_elem_empty =>
+            have := Set.mem_empty_iff_false x
+            apply this.mp
+            exact h_x_elem_empty
+      | inr h_elem_removeCell =>
+        simp [removeCell] at h_elem_removeCell
+        have := Set.diff_subset split {targetCell}
+        have h_empty_not_mem_diff := Set.not_mem_subset this h
+        have h_empty_mem_diff := (castSucc_empty_elem_iff (split \ {targetCell})).mp h_elem_removeCell
+        contradiction
+
+theorem insertLastAt_is_disjoint_insert {n : ℕ} (split : Split n) (targetCell : Cell n)
+  : Disjoint {targetCell.insertLast} (split.removeCell targetCell).castSucc := by
+    apply disjoint_iff.mpr
+    simp [removeCell, castSucc, Fin.castSucc]
+    intro cell _ _
+    have h_k : ¬ (∀ (x : Fin (n + 1)), x ∈ cell.castSucc ↔ x ∈ targetCell.insertLast) := by
+      simp [not_iff]
+      exists (Fin.last n)
+      constructor
+      · intro
+        simp [Cell.insertLast]
+      · intro
+        apply Set.disjoint_singleton_left.mp
+        exact Cell.insertLast_is_disjoint_insert cell
+    have := Set.ext_iff (s := cell.castSucc) (t := targetCell.insertLast)
+    exact (not_congr this).mpr h_k
+
+-- Helper prop
+def InSplitInsertLastAtAndContainsLast {n : ℕ} (split : Split n) (targetCell : Cell n) (cell : Cell (n + 1)) : Prop
+  := cell ∈ split.insertLastAt targetCell ∧ Fin.last n ∈ cell
+
+theorem exists_contains_last {n : ℕ} (split : Split n) (targetCell : Cell n)
+  : ∃ (cell : Cell (n + 1)), InSplitInsertLastAtAndContainsLast split targetCell cell := by
+    simp [InSplitInsertLastAtAndContainsLast, insertLastAt, Set.insert, Cell.insertLast]
+
+theorem last_not_mem_of_mem_removeCell_castSucc {n : ℕ} (split : Split n) (targetCell : Cell n) (cell : Cell (n + 1)) (h : cell ∈ (split.removeCell targetCell).castSucc)
+  : Fin.last n ∉ cell := by
+    simp [removeCell, castSucc, Fin.castSucc] at h
+    cases h with
+      | intro cell_pre h_cell_pre =>
+        rw [← h_cell_pre.right]
+        simp [Cell.castSucc]
+        intro x _
+        exact Fin.ne_of_lt (Fin.castSucc_lt_last x)
+
+theorem unique_contains_last {n : ℕ} (split : Split n) (targetCell : Cell n)
+  : ∀ (cell₁ cell₂ : Cell (n + 1)), InSplitInsertLastAtAndContainsLast split targetCell cell₁ → InSplitInsertLastAtAndContainsLast split targetCell cell₂ → cell₁ = cell₂ := by
+    intros cell₁ cell₂ h₁ h₂
+    simp [InSplitInsertLastAtAndContainsLast, insertLastAt, Set.insert] at *
+    -- TODO: Factor out into lemma to not have to repeat this stuff
+    have h_cell₁ : cell₁ = targetCell.insertLast := by
+      have h_not_in_right : cell₁ ∉ (split.removeCell targetCell).castSucc := by
+        -- TODO: Maybe we can do this without by_contra (since it isn't constructive is it?)
+        by_contra h_in_right
+        have h_last_not_mem := last_not_mem_of_mem_removeCell_castSucc split targetCell cell₁ h_in_right
+        have h_last_mem := h₁.right
+        contradiction
+      apply (or_iff_left (a := cell₁ = targetCell.insertLast) (b := cell₁ ∈ (split.removeCell targetCell).castSucc) h_not_in_right).mp
+      exact h₁.left
+    have h_cell₂ : cell₂ = targetCell.insertLast := by
+      have h_not_in_right : cell₂ ∉ (split.removeCell targetCell).castSucc := by
+        by_contra h_in_right
+        have h_last_not_mem := last_not_mem_of_mem_removeCell_castSucc split targetCell cell₂ h_in_right
+        have h_last_mem := h₂.right
+        contradiction
+      apply (or_iff_left (a := cell₂ = targetCell.insertLast) (b := cell₂ ∈ (split.removeCell targetCell).castSucc) h_not_in_right).mp
+      exact h₂.left
+    rw [h_cell₁, h_cell₂]
+
+-- NOTE: This can be used in insertLast'_produces_partitions
+theorem insertLastAt_unique_cell_last_mem {n : ℕ} (split : Split n) (targetCell : Cell n)
+  : ∃! (cell : Cell (n + 1)), InSplitInsertLastAtAndContainsLast split targetCell cell
+    := exists_unique_of_exists_of_unique (exists_contains_last split targetCell) (unique_contains_last split targetCell)
+
+theorem insertLastAt_castSucc_mem_of_mem_of_ne_targetCell
+    {n : ℕ}
+    {split : Split n}
+    {targetCell : Cell n}
+    {cell : Cell n}
+    (h_mem : cell ∈ split)
+    (h_ne : cell ≠ targetCell)
+  : cell.castSucc ∈ split.insertLastAt targetCell := by
+    simp [insertLastAt, Set.insert, Split,castSucc]
+    right
+    exists cell
+
+-- TODO: Maybe we can find a better name yet (it's alright, but not totally satisfactory).
+-- TODO: Do we even need this if we have the version below?
+def insertLast {n : ℕ} (split : Split n) : Set (Split (n + 1))
+  := {split.insertLastAt cell | cell ∈ split.insert ∅}
+
+theorem insertLastAt_mapsTo {n : ℕ} (split : Split n)
+  : Set.MapsTo split.insertLastAt (split.insert ∅) split.insertLast := by
+    simp [Set.MapsTo, insertLast]
+    intro cell cell_mem_split
+    exists cell
+
+-- TODO: Use insertLastAt_mapsTo here
+theorem insertLastAt_surjOn {n : ℕ} (split : Split n)
+  : Set.SurjOn split.insertLastAt (split.insert ∅) split.insertLast := by
+    simp [Set.SurjOn, insertLast, Set.image]
+    intro cell cell_mem_split'
+    exists cell
+
+theorem insertLastAt_bijOn {n : ℕ} (split : Split n)
+  : Set.BijOn split.insertLastAt (split.insert ∅) split.insertLast := by
+    split_ands
+    · exact insertLastAt_mapsTo split
+    · exact insertLastAt_injOn split
+    · exact insertLastAt_surjOn split
+
+theorem insertLast_nonempty_of_mem
+  {n : ℕ}
+  {split : Split n}
+  {split' : Split (n + 1)}
+  (h : split' ∈ insertLast split)
+  : split'.Nonempty := by
+    simp [insertLast] at h
+    cases h with
+      | intro cell h_cell =>
+        rw [← h_cell.right]
+        exact insertLastAt_nonempty _ _
+
+def insertLast' {n : ℕ} (h : n > 0) (split : Split (n - 1)) : Set (Split n)
+  := cast (Nat.sub_add_cancel h) '' split.insertLast
+
+theorem insertLast'_nonempty_of_mem
+  {n : ℕ}
+  {h : n > 0}
+  {split : Split (n - 1)}
+  {split' : Split n}
+  (h : split' ∈ insertLast' h split)
+  : split'.Nonempty := by
+    simp [insertLast'] at h
+    cases h with
+      | intro split'' h_split'' =>
+        rw [← h_split''.right]
+        have h_split''_nonempty : split''.Nonempty := insertLast_nonempty_of_mem h_split''.left
+        simp [cast_nonempty_iff, h_split''_nonempty]
+
+def IsPartition {n : ℕ} (split : Split n) : Prop
+  := Setoid.IsPartition split
+
+end Split
